@@ -1,0 +1,10 @@
+/-
+`iinit`'s interface, instantiated from its proof.
+-/
+import Xv6.ProofIinit
+
+namespace Xv6
+
+theorem Iinit (IL : INITLOCK) (IS : INITSLEEPLOCK) : IINIT := iinit_proof IL IS
+
+end Xv6
